theories/TM/L/Compiler/Compiler_facts.v
@@ -17,6 +17,15 @@ Import VectorNotations.
 From Undecidability.TM.L.Compiler Require Import Compiler_spec.
 
 Require Import Equations.Prop.DepElim.
+      
+Definition L_computable_bool_closed {k} (R : Vector.t (list bool) k -> (list bool) -> Prop) := 
+  exists s, closed s /\ forall v : Vector.t (list bool) k, 
+      (forall m, R v m <-> L.eval (Vector.fold_left (fun s n => L.app s (encL n)) s v) (encL m)) /\
+      (forall o, L.eval (Vector.fold_left (fun s n => L.app s (encL n)) s v) o -> exists m, o = encL m).
+
+Lemma L_computable_bool_can_closed k R:
+  L_computable_bool_closed R <-> L_computable (k:=k) R.
+Admitted.
 
 Lemma nth_error_to_list {X n} (v : Vector.t X n) i k :
   k = (proj1_sig (Fin.to_nat i)) ->
