theories/TM/L/Eval.v
@@ -1,0 +1,149 @@
+From Undecidability Require Import L.Datatypes.LBool L.Datatypes.Lists L.Tactics.LTactics L.Util.L_facts.
+
+Require Import Undecidability.Shared.Libs.PSL.FiniteTypes.FinTypes Undecidability.Shared.Libs.PSL.Vectors.Vectors.
+Require Import List.
+
+Require Import Undecidability.TM.Util.TM_facts.
+
+From Undecidability Require Import ProgrammingTools LM_heap_def WriteValue CaseList Copy ListTM  JumpTargetTM WriteValue Hoare.
+From Undecidability.TM.L Require Import Alphabets M_LHeapInterpreter.
+From Undecidability Require Import TM.TM L.AbstractMachines.FlatPro.LM_heap_correct.
+
+From Undecidability Require Import L.L TM.TM.
+Require Import List.
+
+Import Vector.VectorNotations.
+Import ListNotations ResourceMeasures.
+
+
+From Undecidability.TM.L Require Import Compiler_spec Compiler_facts UnfoldClos Compiler.AddToBase.
+
+Require Import Equations.Prop.DepElim.
+
+Import CasePair Code.CaseList.
+
+Set Default Proof Using "Type".
+
+
+Module EvalL.
+Section Fix.
+
+  Variable Σ : finType.
+
+  Definition Σintern :Type := sigStep + sigList (sigPair sigHClos sigNat).
+
+
+  Context (retr_eval : Retract Σintern Σ) (retr_pro : Retract sigPro Σ).
+
+
+  Definition retr_unfolder : Retract (sigList (sigPair sigHClos sigNat)) Σ := ComposeRetract retr_eval _.
+  Definition retr_interpreter : Retract sigStep Σ := ComposeRetract retr_eval _.
+
+  Local Instance retr_closs_intrp : Retract (sigList (sigHClos)) Σ := ComposeRetract retr_interpreter _.
+  Local Instance retr_clos_intrp : Retract sigHClos Σ := ComposeRetract retr_closs_intrp _.
+  Local Instance retr_pro_intrp : Retract sigPro Σ := ComposeRetract retr_clos_intrp _.
+  
+  Local Instance retr_nat_clos_ad' : Retract sigNat sigHClos := Retract_sigPair_X _ (Retract_id _).
+  Local Instance retr_nat_clos_ad : Retract sigNat Σ := ComposeRetract _ retr_nat_clos_ad'.
+  Local Instance retr_heap : Retract sigHeap Σ := ComposeRetract retr_interpreter _.
+
+
+  (*
+    auxiliary tapes:
+
+    0    : T
+    1    : V
+    2    : H
+    3-4  : aux for init
+    5-12 : aux for loop
+    13   : t
+   *)
+   
+  Definition M : pTM (Σ^+) unit 11 :=
+    Translate retr_pro retr_pro_intrp @ [|Fin0|];;
+    CopyValue _ @ [|Fin0;Fin1|];;
+    Reset _ @[|Fin0|];;
+    WriteValue 0 ⇑ retr_nat_clos_ad @ [| Fin0|];;
+    Constr_pair _ _ ⇑ retr_clos_intrp @ [|Fin0;Fin1|];;
+    Reset _ @ [|Fin0|];;
+    WriteValue ( []%list) ⇑ retr_closs_intrp @ [| Fin0|];;
+    Constr_cons _ ⇑ retr_closs_intrp @ [|Fin0;Fin1|];;
+    Reset _ @ [|Fin1|];;
+    WriteValue ( []%list) ⇑ retr_closs_intrp @ [| Fin1|];;
+    WriteValue ( []%list ) ⇑ retr_heap @ [| Fin2|];;
+    M_LHeapInterpreter.Loop ⇑ retr_interpreter;;
+    Reset _ @ [|Fin0|];;
+    CaseList _ ⇑ retr_closs_intrp @ [| Fin1;Fin0 |];;
+    Reset _ @ [|Fin1|];;
+    UnfoldClos.M retr_unfolder retr_heap retr_clos_intrp @ [| Fin0;Fin2;Fin1;Fin3;Fin4;Fin5;Fin6;Fin7;Fin8;Fin9|];;
+    Reset _ @ [|Fin2|];;
+    Translate (UnfoldClos.retr_pro _) retr_pro @ [|Fin0|].
+
+  
+  Arguments "+" : simpl never.
+  Arguments "*" : simpl never.
+
+  Lemma SpecT' s k t:
+   closed s -> evalIn k s t ->
+   exists k0,
+    TripleT ≃≃([],[|Contains retr_pro (compile s)|] ++ Vector.const Void _)
+      k0 M
+      (fun _ => ≃≃([],[|Contains retr_pro (compile t)|] ++ Vector.const Void _)).
+  Proof.
+    intros cls HR%timeBS_evalIn.
+    eapply completenessTime in HR as (?&?&?&?). 2:easy.
+    eexists.
+    unfold M.
+    do 11 (hstep_seq;[]). cbn.
+    hstep_seq;[| | ] .
+    { refine (TripleT_RemoveSpace _). intros. eapply Interpreter_SpecT. eassumption. inversion 1. }
+    now cbn; tspec_ext.
+    do 2 (hstep_seq;[]).
+    hintros _ _.
+    hstep_seq;[].
+    hstep_seq;[|].
+    { eapply UnfoldClos.SpecT. eassumption. }
+    cbn.
+    do 2 (hstep_seq;[]). reflexivity.
+  Qed.
+
+  
+  Lemma Spec' s :
+   closed s -> 
+    Triple ≃≃([],[|Contains retr_pro (compile s)|] ++ Vector.const Void _)
+      M
+      (fun _ t => exists s', t ≃≃ ([s ⇓ s']%list,[|Contains retr_pro (compile s')|] ++ Vector.const Void _)).
+  Proof.
+    intros cls.
+    unfold M.
+    do 11 (hstep_seq;[]). cbn.
+    hstep.
+    {
+      eapply Consequence with (Q1:= fun y => _) (Q2:= fun y => _).
+      eapply ChangeAlphabet_Spec_ex with (Q:= fun y x => _) (Q':= fun y x => _) (Ctx:= fun x (H:Prop) => (steps_k (snd x) _ (fst x) /\ halt_state (fst x)) /\
+        (fst (fst (fst x)) = []%list ->
+        H)).
+      now refine (Interpreter_Spec [(0,compile s)] [] [])%list. now unfold "==>",Proper,Basics.impl. now cbn; tspec_ext. cbn;intros _. apply reflexivity.
+    }
+    cbn. intros _.
+    eapply Triple_exists_pre. intros [[[T' V'] H'] k'];cbn.
+    eapply Triple_and_pre. intros [HR Hhalt].
+    unfold steps_k in*.
+    edestruct soundness with (1:=cls) as (?&?&?&Heq&?&?). {split. now eapply pow_star. eassumption. }
+    injection Heq as [= -> -> ->].
+    eapply Triple_forall_pre. exists eq_refl.
+    do 2 (hstep_seq;[]).
+    hintros ? _.
+    do 2 hstep_seq;[|].
+    { refine (TripleT_Triple _). refine (UnfoldClos.SpecT _ _ _ _). eassumption. }
+    cbn.
+    hstep_seq.
+    eapply Triple_exists_con. eexists _.
+    change (fun x => ?h x) with h.
+    eapply Consequence_post.
+    now hsteps_cbn.
+    cbn. intros _. tspec_ext. easy.
+  Qed.
+
+End Fix.
+End EvalL.
